regalloc: loop through srcvars by increasing life length,
and assign each srcvar to the lowest impvar which is still free
during the whole lifespan of the srcvar.
This avoids spilling of short-lived temporaries.
For current garage door code in fiat-crypto, this reduces the total
instruction count from 8483 to 7259 (almost -15%).

compiler/src/compiler/RegAlloc.v
@@ -142,6 +142,9 @@ Definition temp_regs : list impvar := Eval compute in List.filter not_reserved (
 Definition saved_regs: list impvar := Eval compute in List.filter not_reserved (reg_class.all reg_class.saved).
 Definition arg_regs  : list impvar := Eval compute in List.filter not_reserved (reg_class.all reg_class.arg).
 
+
+(* ** Previous implementation: assign impvars in one scan over the events *)
+
 (* Register availability, split by how preferable they are.
    For simplicity, we use the argument registers *only* for argument passing and as spilling temporaries. *)
 Record av_regs := mk_av_regs {
@@ -209,6 +212,110 @@ Fixpoint process_intervals(corresp: list (srcvar * impvar))(av: av_regs)(l: list
       process_intervals corresp av rest
   | nil => corresp
   end.
+
+
+(* ** New implementation: Process source variables from shortest to longest lifetime *)
+
+(* varname, start time, live interval length *)
+Definition lifetime := (string * (Z * Z))%type.
+
+Definition non_overlapping: lifetime -> lifetime -> bool :=
+  fun '(_, (start1, len1)) '(_, (start2, len2)) =>
+    if start1 + len1 <? start2 then true else start2 + len2 <? start1.
+
+(* custom implementation because List.forallb is not short-circuiting *)
+Section ConflictFree.
+  Context (candidate: lifetime).
+  Fixpoint conflict_free(occ: list lifetime): bool :=
+    match occ with
+    | nil => true
+    | l :: tail => if non_overlapping candidate l then conflict_free tail else false
+    end.
+End ConflictFree.
+
+(* i-th element contains list of intervals during which i-th impvar is occupied *)
+Definition occupancy := list (list lifetime).
+
+Fixpoint assign_srcvar(occs: occupancy)(v: lifetime): occupancy :=
+  match occs with
+  | occ :: tail => if conflict_free v occ then ((v :: occ) :: tail)
+                   else occ :: assign_srcvar tail v
+  | nil => [ [v] ] (* start using next (so far unused) register or stack slot *)
+  end.
+
+Section Sorting.
+  Context {A: Type} (lt: A -> A -> bool).
+
+  Section WithA.
+    Context (a: A).
+    Fixpoint insert_into_sorted(l: list A): list A :=
+      match l with
+      | [] => [a]
+      | h :: t => if lt a h then a :: l else h :: (insert_into_sorted t)
+      end.
+  End WithA.
+
+  Definition sort: list A -> list A := List.fold_right insert_into_sorted nil.
+End Sorting.
+
+Definition compare_interval_length: lifetime -> lifetime -> bool :=
+  fun '(name1, (start1, len1)) '(name2, (start2, len2)) => Z.ltb len1 len2.
+
+Section IndexOf.
+  Context {A: Type} (predicate: A -> bool).
+  Fixpoint index_of(l: list A): Z :=
+    match l with
+    | [] => -1
+    | h :: t => if predicate h then 0 else
+                  let rec := index_of t in
+                  match rec with
+                  | Zneg _ => rec
+                  | _ => rec + 1
+                  end
+    end.
+End IndexOf.
+
+Goal index_of (Z.eqb 3) [4; 3; 1] = 1. cbv. reflexivity. Abort.
+Goal index_of (Z.eqb 3) [4; 4; 1] = -1. cbv. reflexivity. Abort.
+
+Fixpoint events_to_intervals(current_time: Z)(events: list event): list lifetime :=
+  match events with
+  | (varname, is_start) :: tail =>
+      let rec := events_to_intervals (current_time + 1) tail in
+      if is_start then
+        let len := 1 + index_of (fun '(varname', _) => String.eqb varname varname') tail in
+        (varname, (current_time, len)) :: rec
+      else rec
+  | nil => nil
+  end.
+
+(* We use registers x6 to x9, registers x18 to x31, and stack slots x32 and beyond *)
+Definition first_available_impvar := 6.
+Definition next_available_impvar(v: Z): Z :=
+  if Z.eqb v 9 then 18 else v + 1.
+
+Fixpoint add_corresp_of_impvar(impvarname: Z)(occ: list lifetime)
+  (corresp: list (srcvar * impvar)): list (srcvar * impvar) :=
+  match occ with
+  | (srcvarname, _) :: tail =>
+      (srcvarname, impvarname) :: add_corresp_of_impvar impvarname tail corresp
+  | nil => corresp
+  end.
+
+Fixpoint corresp_of_impvars(start_impvar: Z)(o: occupancy): list (srcvar * impvar) :=
+  match o with
+  | h :: t => add_corresp_of_impvar start_impvar h
+                (corresp_of_impvars (next_available_impvar start_impvar) t)
+  | nil => nil
+  end.
+
+Definition events_to_corresp(events: list event): list (srcvar * impvar) :=
+  let sorted_intervals := sort compare_interval_length (events_to_intervals 0 events) in
+  let occ := List.fold_left assign_srcvar sorted_intervals [] in
+  corresp_of_impvars first_available_impvar occ.
+
+
+(* ** Common: Applying a rename mapping (corresp) *)
 
 Definition rename_bcond(corresp: list (srcvar * impvar))(c: bcond): result bcond' :=
   match c with
@@ -370,7 +477,8 @@ End WithBugs.
 
 Definition regalloc_function: list srcvar * list srcvar * stmt -> result (list impvar * list impvar * stmt') :=
   fun '(args, rets, fbody) =>
-    let corresp := process_intervals [] initial_av_regs (intervals args fbody rets) in
+  (*let corresp := process_intervals [] initial_av_regs (intervals args fbody rets) in*)
+    let corresp := events_to_corresp (intervals args fbody rets) in
     fbody' <- rename corresp fbody;;
     args' <- lookups args corresp;;
     rets' <- lookups rets corresp;;
@@ -734,7 +842,7 @@ Proof.
   eapply defuel_loop_inv'; eassumption.
 Qed.
 
-Section RegAlloc.
+Section CheckerCorrect.
 
   Context {width} {BW: Bitwidth width} {word: word.word width} {word_ok: word.ok word}.
   Context {mem: map.map word byte}.
@@ -1045,4 +1153,4 @@ Section RegAlloc.
       eapply exec.skip. eauto.
   Qed.
 
-End RegAlloc.
+End CheckerCorrect.
